<?xml version="1.0" encoding="utf-8"?>
<rdf:RDF
   xmlns:owl="http://www.w3.org/2002/07/owl#"
   xmlns:rdf="http://www.w3.org/1999/02/22-rdf-syntax-ns#"
   xmlns:rdfs="http://www.w3.org/2000/01/rdf-schema#"
>
  <rdf:Description rdf:about="https://vocabularies.wholetale.org/wt/1.0/usesDataset">
    <rdf:type rdf:resource="http://www.w3.org/2002/07/owl#ObjectProperty"/>
    <rdfs:domain rdf:resource="https://vocabularies.wholetale.org/wt/1.0/Tale"/>
    <rdfs:range rdf:resource="https://schema.org/Dataset"/>
    <rdfs:comment xml:lang="en">Relates a Tale with external data.</rdfs:comment>
    <rdfs:label xml:lang="en">Uses Dataset</rdfs:label>
  </rdf:Description>
  <rdf:Description rdf:about="https://vocabularies.wholetale.org/wt/1.0/">
    <rdf:type rdf:resource="http://www.w3.org/2002/07/owl#Ontology"/>
    <owl:versionIRI rdf:resource="https://vocabularies.wholetale.org/wt/1.0/"/>
    <rdfs:comment xml:lang="en">This document defines a language for describing Tale related objects and the relations between them.</rdfs:comment>
    <rdfs:label xml:lang="en">Whole Tale Ontology</rdfs:label>
    <owl:versionInfo>Version 1.0</owl:versionInfo>
  </rdf:Description>
  <rdf:Description rdf:about="https://vocabularies.wholetale.org/wt/1.0/size">
    <rdf:type rdf:resource="http://www.w3.org/2002/07/owl#ObjectProperty"/>
    <rdfs:domain rdf:resource="http://www.openarchives.org/ore/terms/AggregatedResource"/>
    <rdfs:range rdf:resource="http://www.w3.org/2001/XMLSchema#integer"/>
    <rdfs:comment xml:lang="en">The size of a file in bytes.</rdfs:comment>
    <rdfs:label xml:lang="en">Size</rdfs:label>
  </rdf:Description>
  <rdf:Description rdf:about="https://vocabularies.wholetale.org/wt/1.0/TaleVersion">
    <rdf:type rdf:resource="http://www.w3.org/2002/07/owl#Class"/>
    <rdfs:subClassOf rdf:resource="https://schema.org/CreativeWork"/>
    <rdfs:comment xml:lang="en">A snapshot of a Tale's state that may be attributed to users that are not first authors of the Tale.</rdfs:comment>
    <rdfs:label xml:lang="en">Tale Version</rdfs:label>
  </rdf:Description>
  <rdf:Description rdf:about="https://vocabularies.wholetale.org/wt/1.0/mimetype">
    <rdf:type rdf:resource="http://www.w3.org/2002/07/owl#ObjectProperty"/>
    <rdfs:domain rdf:resource="http://www.openarchives.org/ore/terms/AggregatedResource"/>
    <rdfs:range rdf:resource="http://www.w3.org/2000/01/rdf-schema#Literal"/>
    <rdfs:comment xml:lang="en">The mimetype of a file.</rdfs:comment>
    <rdfs:label xml:lang="en">Mimetype</rdfs:label>
  </rdf:Description>
  <rdf:Description rdf:about="https://vocabularies.wholetale.org/wt/1.0/Tale">
    <rdf:type rdf:resource="http://www.w3.org/2002/07/owl#Class"/>
    <rdfs:subClassOf rdf:resource="http://purl.org/wf4ever/ro#ResearchObject"/>
    <rdfs:subClassOf rdf:resource="https://schema.org/CreativeWork"/>
    <rdfs:comment xml:lang="en">A collection of data, code, and metadata that together define and describe a computational experiment.</rdfs:comment>
    <rdfs:label xml:lang="en">Tale</rdfs:label>
  </rdf:Description>
  <rdf:Description rdf:about="https://vocabularies.wholetale.org/wt/1.0/md5">
    <rdf:type rdf:resource="http://www.w3.org/2002/07/owl#ObjectProperty"/>
    <rdfs:domain rdf:resource="http://www.openarchives.org/ore/terms/AggregatedResource"/>
    <rdfs:range rdf:resource="http://www.w3.org/2000/01/rdf-schema#Literal"/>
    <rdfs:comment xml:lang="en">The MD5 checksum of a file.</rdfs:comment>
    <rdfs:label xml:lang="en">MD5 Checksum</rdfs:label>
  </rdf:Description>
  <rdf:Description rdf:about="https://vocabularies.wholetale.org/wt/1.0/identifier">
    <rdf:type rdf:resource="http://www.w3.org/2002/07/owl#ObjectProperty"/>
    <rdfs:domain rdf:resource="https://vocabularies.wholetale.org/wt/1.0/Tale"/>
    <rdfs:domain rdf:resource="http://www.openarchives.org/ore/terms/AggregatedResource"/>
    <rdfs:range rdf:resource="http://www.w3.org/2000/01/rdf-schema#Literal"/>
    <rdfs:comment xml:lang="en">An identifier used by the internal Whole Tale system for resources.</rdfs:comment>
    <rdfs:label xml:lang="en">Identifier</rdfs:label>
  </rdf:Description>
</rdf:RDF>
